termination proofs is a pita
Signed-off-by: Shaobo He <shaobohe@amazon.com>

cedar-lean/Cedar/Thm/Validation/WellTyped/TypeLifting.lean
@@ -18,6 +18,7 @@ import Cedar.Validation.TypedExpr
 import Cedar.Spec
 import Cedar.Thm.Validation
 import Cedar.Thm.Validation.Typechecker.Record
+import Cedar.Thm.Validation.Typechecker.Types
 import Cedar.Thm.Data
 
 /-!
@@ -86,38 +87,226 @@ theorem type_lifting_preserves_evaluation_results {x : TypedExpr} {request : Req
  := by
  simp only [type_lifting_preserves_expr x]
 
+inductive Lifted : CedarType → CedarType → Prop
+  | bool {bty : BoolType} :
+    Lifted (.bool bty) (.bool .anyBool)
+  | int :
+    Lifted .int .int
+  | string :
+    Lifted .string .string
+  | entity {ety : EntityType} :
+    Lifted (.entity ety) (.entity ety)
+  | ext {extTy : ExtType} :
+    Lifted (.ext extTy) (.ext extTy)
+  | set {ty₁ ty₂ : CedarType}
+    (h : Lifted ty₁ ty₂) :
+    Lifted (.set ty₁) (.set ty₂)
+  | record_nil :
+    Lifted (.record (.mk [])) (.record (.mk []))
+  | record_fst_optional {ty₁ ty₂ : CedarType} {k : Attr} {m₁ m₂ : List (Attr × QualifiedType)}
+    (h₁ : Lifted ty₁ ty₂)
+    (h₂ : Lifted (.record (.mk m₁)) (.record (.mk m₂))) :
+    Lifted (.record (.mk ((k, .optional ty₁) :: m₁))) (.record (.mk ((k, .optional ty₂) :: m₂)))
+  | record_fst_required {ty₁ ty₂ : CedarType} {k : Attr} {m₁ m₂ : List (Attr × QualifiedType)}
+    (h₁ : Lifted ty₁ ty₂)
+    (h₂ : Lifted (.record (.mk m₁)) (.record (.mk m₂))) :
+    Lifted (.record (.mk ((k, .required ty₁) :: m₁))) (.record (.mk ((k, .required ty₂) :: m₂)))
+
+mutual
+
+theorem lifted_record_is_lifted (m : List (Attr × QualifiedType)) :
+  Lifted (.record (.mk m)) (.record (.mk (CedarType.liftBoolTypesRecord m)))
+:= by
+  unfold CedarType.liftBoolTypesRecord
+  split
+  case _ => exact Lifted.record_nil
+  case _ qty l =>
+    unfold QualifiedType.liftBoolTypes
+    split
+    case _ ty =>
+      have hᵢ₁ := lifted_type_is_lifted ty
+      have hᵢ₂ := lifted_record_is_lifted l
+      exact Lifted.record_fst_optional hᵢ₁ hᵢ₂
+    case _ ty =>
+      have hᵢ₁ := lifted_type_is_lifted ty
+      have hᵢ₂ := lifted_record_is_lifted l
+      exact Lifted.record_fst_required hᵢ₁ hᵢ₂
+
+theorem lifted_type_is_lifted (ty : CedarType) :
+  Lifted ty ty.liftBoolTypes
+:= by
+  cases ty <;> simp [CedarType.liftBoolTypes]
+  case bool =>
+    simp [BoolType.lift]
+    exact Lifted.bool
+  case int =>
+    exact Lifted.int
+  case string =>
+    exact Lifted.string
+  case entity =>
+    exact Lifted.entity
+  case ext =>
+    exact Lifted.ext
+  case set ty' =>
+    have := lifted_type_is_lifted ty'
+    exact Lifted.set this
+  case record rty =>
+    unfold CedarType.liftBoolTypesRecord
+    split
+    case _ heq =>
+      have : rty = (Data.Map.mk []) := by
+        simp [Data.Map.kvs_nil_iff_empty, Data.Map.empty] at heq
+        exact heq
+      simp [this]
+      exact Lifted.record_nil
+    case _ a qt l heq =>
+      have : rty = (Data.Map.mk ((a, qt)::l)) := by
+        cases rty
+        simp at heq
+        simp [heq]
+      simp [this]
+      clear this
+      unfold QualifiedType.liftBoolTypes
+      split
+      case _ ty' =>
+        have hᵢ := lifted_type_is_lifted ty'
+        exact Lifted.record_fst_optional hᵢ (lifted_record_is_lifted l)
+      case _ ty' =>
+        have hᵢ := lifted_type_is_lifted ty'
+        exact Lifted.record_fst_required hᵢ (lifted_record_is_lifted l)
+end
+
+theorem lifted_type_is_super_type {ty₁ ty₂ : CedarType} :
+  Lifted ty₁ ty₂ → subty ty₁ ty₂
+:= by
+  intro h
+  induction h
+  case bool =>
+    simp [subty, lub?, lubBool]
+  case int =>
+    simp [subty, lub?]
+  case string =>
+    simp [subty, lub?]
+  case entity =>
+    simp [subty, lub?]
+  case ext =>
+    simp [subty, lub?]
+  case set h hᵢ =>
+    simp only [subty] at hᵢ
+    simp only [subty, lub?]
+    split at hᵢ
+    case _ heq =>
+      simp [heq, hᵢ]
+    case _ => cases hᵢ
+  case record_nil =>
+    simp [subty, lub?, lubRecordType]
+  case record_fst_optional hᵢ₁ hᵢ₂ =>
+    simp [subty, lub?]
+    simp [subty] at hᵢ₁
+    simp [subty, lub?] at hᵢ₂
+    split at hᵢ₁
+    case _ heq =>
+      split at hᵢ₂
+      case _ m₁ m₂ _ _ _ _ _ _ heq₁ =>
+        simp [lubRecordType, lubQualifiedType, heq]
+        simp at hᵢ₂
+        simp [hᵢ₂] at heq₁
+        generalize h : lubRecordType m₁ m₂ = res
+        cases res
+        case none =>
+          simp [h] at heq₁
+        case some =>
+          simp [h] at heq₁
+          simp [h, hᵢ₁, heq₁]
+      case _ => cases hᵢ₂
+    case _ => cases hᵢ₁
+  case record_fst_required hᵢ₁ hᵢ₂ =>
+    simp [subty, lub?]
+    simp [subty] at hᵢ₁
+    simp [subty, lub?] at hᵢ₂
+    split at hᵢ₁
+    case _ heq =>
+      split at hᵢ₂
+      case _ m₁ m₂ _ _ _ _ _ _ heq₁ =>
+        simp [lubRecordType, lubQualifiedType, heq]
+        simp at hᵢ₂
+        simp [hᵢ₂] at heq₁
+        generalize h : lubRecordType m₁ m₂ = res
+        cases res
+        case none =>
+          simp [h] at heq₁
+        case some =>
+          simp [h] at heq₁
+          simp [h, hᵢ₁, heq₁]
+      case _ => cases hᵢ₂
+    case _ => cases hᵢ₁
+
+  /-
+  unfold CedarType.liftBoolTypes
+  split <;> unfold lub?
+  case _ =>
+    simp only [lubBool, BoolType.lift, Option.some.injEq, CedarType.bool.injEq, ite_eq_right_iff,
+      imp_self]
+  case _ =>
+    simp only [lifted_type_is_super_type, Option.bind_some_fun]
+  case _ m =>
+    simp only [do_some]
+    induction m
+    case nil =>
+      simp only [CedarType.liftBoolTypesRecord, lubRecordType, Option.some.injEq, List.nil_eq,
+        CedarType.record.injEq, Data.Map.mk.injEq, and_self, exists_eq]
+    case cons hᵢ =>
+      simp at hᵢ
+      simp
+      unfold lubRecordType
+      split
+      case _ heq _ =>
+        simp only [reduceCtorEq] at heq
+      case _ head tail _ _ k₁ v₁ _ k₂ v₂ _ h₁ h₂ =>
+        simp [CedarType.liftBoolTypesRecord] at h₂
+        rcases h₂ with ⟨⟨h₂₁, h₂₂⟩, h₂₃⟩
+        simp only [List.cons.injEq] at h₁
+        rcases h₁ with ⟨h₁₁, h₁₂⟩
+        have h : head = (head.fst, head.snd) := by rfl
+        rw [h] at h₁₁
+        clear h
+        simp at h₁₁
+        rcases h₁₁ with ⟨h₁₃, h₁₄⟩
+        have h : lubQualifiedType v₁ v₂ = v₂ := by
+          unfold lubQualifiedType
+          split
+          case _ ty₁ ty₂ =>
+            simp [h₁₄] at h₂₂
+            simp [QualifiedType.liftBoolTypes] at h₂₂
+            rw [←h₂₂]
+            simp only [lifted_type_is_super_type, Option.bind_some_fun]
+          case _ ty₁ ty₂ =>
+            simp [h₁₄] at h₂₂
+            simp [QualifiedType.liftBoolTypes] at h₂₂
+            rw [←h₂₂]
+            simp only [lifted_type_is_super_type, Option.bind_some_fun]
+          case _ => sorry
+        rw [←h₂₁, ←h₁₃]
+        simp only [bne_self_eq_false, Bool.false_eq_true, ↓reduceIte, h, ← h₁₂, ← h₂₃, hᵢ,
+          Option.bind_some_fun, Option.some.injEq]
+        rw [←h₂₂]
+        simp only [CedarType.liftBoolTypesRecord]
+      case _ h => sorry
+  case _ =>
+    sorry
+-/
+
 theorem type_lifting_preserves_instance_of_type {v : Value} {ty : CedarType} :
   InstanceOfType v ty →
   InstanceOfType v ty.liftBoolTypes
 := by
-  intro h₁
-  induction h₁ <;> simp only [CedarType.liftBoolTypes]
-  case instance_of_bool =>
-    simp only [BoolType.lift, bool_is_instance_of_anyBool]
-  case instance_of_int =>
-    exact InstanceOfType.instance_of_int
-  case instance_of_string =>
-    exact InstanceOfType.instance_of_string
-  case instance_of_entity e ety h =>
-    exact InstanceOfType.instance_of_entity e ety h
-  case instance_of_set s tyᵢ _ hᵢ =>
-    exact InstanceOfType.instance_of_set s tyᵢ.liftBoolTypes hᵢ
-  case instance_of_record r rty hᵢ₁ hᵢ₂ hᵢ₃ hᵢ₄ =>
-    apply InstanceOfType.instance_of_record
-    case h₁ =>
-      intro k h₂
-      replace hᵢ₁ := hᵢ₁ k h₂
-      simp only [List.map₁_eq_map
-          (fun (x : Attr × QualifiedType) => (x.fst, QualifiedType.liftBoolTypes x.snd))]
-      simp [Data.Map.contains, Data.Map.find?, Data.Map.make, Data.Map.kvs]
-      sorry
-    case h₂ =>
-      intro k v qty h₂
-      replace hᵢ₄ := λ qty => hᵢ₄ k v qty h₂
-      sorry
-    case h₃ =>
-      sorry
-  case instance_of_ext x xty hᵢ =>
-    exact InstanceOfType.instance_of_ext x xty hᵢ
-
+  intro h
+  have h' := @lifted_type_is_super_type ty ty.liftBoolTypes (lifted_type_is_lifted ty)
+  simp [subty] at h'
+  split at h'
+  case _ heq =>
+    simp at h'
+    simp [h'] at heq
+    exact @instance_of_lub_left v ty.liftBoolTypes ty ty.liftBoolTypes heq h
+  case _ => cases h'
 end Cedar.Thm
